tried to prove preservation lemma

theories/Lambda.v
@@ -3,6 +3,90 @@ From Autosubst Require Import Autosubst.
 Check subst_comp.
 
 Inductive term : Type :=
-| Var (n : nat)
+| Var (n : var)
 | App (s t : term)
 | Lam (s : {bind term}).
+
+Instance Ids_term : Ids term. derive. Defined.
+Instance Rename_term : Rename term.  derive. Defined.
+Instance Subst_term : Subst term. derive. Defined.
+
+Instance SubstLemmas_term : SubstLemmas term. derive. Defined.
+
+Lemma var_subst:
+  forall (x:var) (sigma : var -> term), (Var x).[sigma] = sigma x.
+Proof.
+  intros x sigma. simpl. reflexivity.
+Qed.
+
+Inductive step : term -> term -> Prop :=
+| Step_beta (s s' t : term) : s' = s.[t .: ids] -> step (App (Lam s) t) s'
+| Step_app1 (s s' t : term) : step s s' -> step (App s t) (App s' t)
+| Step_app2 (s t t' : term) : step t t' -> step (App s t) (App s t')
+| Step_lam (s s' : term) : step s s' -> step (Lam s) (Lam s').
+
+Lemma step_subst :
+  forall (t t' : term) (sigma : var -> term),
+    step t t' -> step t.[sigma] t'.[sigma].
+Proof.
+  induction t; intros t' sigma Hstep.
+  - inversion Hstep.
+  - inversion Hstep; subst.
+    + simpl. constructor. asimpl. reflexivity.
+    + simpl. constructor. auto.
+    + simpl. constructor. auto.
+  - inversion Hstep. subst. simpl.
+    constructor. auto.
+Qed.
+
+Inductive type :=
+| Base
+| Arr (A B : type).
+
+Inductive types (Gamma : var -> type) : term -> type -> Prop :=
+| Types_var (x : var) (A : type) : Gamma x = A -> types Gamma (Var x) A
+| Types_app (s t : term) (A B : type) :
+  types Gamma s (Arr A B) -> types Gamma t A ->
+  types Gamma (App s t) B
+| Types_lam (s : term) (A B : type) : types (A .: Gamma) s B -> types Gamma (Lam s) (Arr A B).
+
+Lemma type_weakening :
+  forall (Gamma : var -> type) (s : term) (A : type),
+    types Gamma s A ->
+    (forall Delta xi, Gamma = xi >>> Delta -> types Delta s.[ren xi] A).
+Proof.
+  intros Gamma s A H. induction H; intros; simpl; econstructor; auto.
+  - rewrite H0 in H. auto.
+  - asimpl. apply IHtypes. rewrite H0. asimpl. reflexivity.
+Qed.
+
+Lemma type_subst :
+  forall (Gamma : var -> type) (s : term) (A : type) (sigma : var -> term),
+    types Gamma s A ->
+    (forall (x:var) (B:type) , Gamma x = B -> types Gamma (sigma x) B) ->
+    types Gamma s.[sigma] A.
+Proof.
+  intros Gamma s. revert Gamma. induction s; intros; simpl.
+  - apply H0. inversion H. subst. reflexivity.
+  - inversion H. subst. eapply Types_app.
+    + apply IHs1.
+      * apply H3.
+      * assumption.
+    + apply IHs2; assumption.
+  - inversion H. subst. constructor. apply IHs.
+    + assumption.
+    + intros. destruct x.
+      * simpl in H1. subst. constructor. reflexivity.
+      * simpl in H1. apply H0 in H1 as E. asimpl.
+        eapply type_weakening.
+        -- apply E.
+        -- asimpl. reflexivity.
+Qed.
+
+Lemma type_pres :
+  forall (Gamma : var -> type) (s t : term) (A : type),
+    types Gamma s A -> step s t -> types Gamma t A.
+Proof.
+  intros Gamma s t A Hty Hstep. induction Hstep.
+  - inversion Hty. inversion H2. subst. Abort.
+       (* substitution lemma not strong enough *)
